Add run_iter and run_invoke proofs

wasm-proofs/Wasm-Proof/Host.thy
@@ -11,16 +11,15 @@ axiomatization where
 and
   to_handle_to_externref[simp]: "to_handle (to_externref y) = y"
 
-definition type0 :: "tf" where 
+definition type0 :: "tf" where [simp]:
   "type0 = Tf [(T_ref T_ext_ref), (T_ref T_ext_ref)] [(T_num T_i32)]"
 
-consts fixpoint_is_equal :: host_func
-
+(* functions and lemmas for translating between isabelle bool and wasm i32*)
 fun bool_to_i32 :: "bool \<Rightarrow> i32" where
   "bool_to_i32 False = (I32.int_of_nat 0)"
 | "bool_to_i32 True = (I32.int_of_nat 1)"
 
-lemma i32_one_ne_zero[simp]:
+lemma i32_one_ne_zero:
   "(I32.lift0 1) \<noteq> I32.lift0 0"
   by transfer simp
 
@@ -34,30 +33,48 @@ proof
     then show ?thesis by auto
   next
     case False
-    then have "bool_to_i32 a = (I32.int_of_nat 0)"  by auto
-    then show ?thesis using assms I32.int_of_nat_def by auto
+    then have "bool_to_i32 a = (I32.int_of_nat 0)" by auto
+    then show ?thesis
+      using I32.int_of_nat_def assms i32_one_ne_zero int_of_nat_i32.abs_eq by auto
   qed
 next
   assume a
   then show "bool_to_i32 a = (I32.int_of_nat 1)" by auto
 qed
 
+lemma bool_to_i32_false:
+  "bool_to_i32 a = (I32.int_of_nat 0) \<longleftrightarrow> \<not>a"
+  by (metis bool_to_i32.elims bool_to_i32_true)
+
+(* Fixpoint APIs exposed to Wasm modules *)
+consts fixpoint_is_equal :: host_func
+
 axiomatization where
+  (* We are stating here that the exposed fixpoint_is_equal is the same as
+     isabelle is_equal given the declared (host from/to externref) and (bool from/to i32) translations *)
   fixpoint_is_equal_impl:
   "host_func_apply_impl s type0 fixpoint_is_equal 
   [(V_ref (ConstRefExtern r1)), (V_ref (ConstRefExtern r2))]
   = Some (s, [V_num (ConstInt32 (bool_to_i32 (is_equal (to_handle r1) (to_handle r2))))])"
 
-term "ConstInt32 (I32.int_of_nat 1)"
-
+(* Helper lemmas for simplifying bool_to_i32 from the axiom statement *)
 lemma fixpoint_is_equal_correct_handle:
   "is_equal h1 h2 \<longleftrightarrow> host_func_apply_impl s type0 fixpoint_is_equal 
   [(V_ref (ConstRefExtern (to_externref h1))), (V_ref (ConstRefExtern (to_externref h2)))] = Some(s, [V_num (ConstInt32 (I32.int_of_nat 1))])"
   using fixpoint_is_equal_impl bool_to_i32_true by auto
+
+lemma fixpoint_is_equal_correct_handle_neq:
+  "\<not>is_equal h1 h2 \<longleftrightarrow> host_func_apply_impl s type0 fixpoint_is_equal 
+  [(V_ref (ConstRefExtern (to_externref h1))), (V_ref (ConstRefExtern (to_externref h2)))] = Some(s, [V_num (ConstInt32 (I32.int_of_nat 0))])"
+  using fixpoint_is_equal_impl bool_to_i32_false by auto
 
 lemma fixpoint_is_equal_correct_externref:
   "is_equal (to_handle r1) (to_handle r2) \<longleftrightarrow> host_func_apply_impl s type0 fixpoint_is_equal 
   [(V_ref (ConstRefExtern r1)), (V_ref (ConstRefExtern r2))] = Some(s, [V_num (ConstInt32 (I32.int_of_nat 1))])"
   using fixpoint_is_equal_impl bool_to_i32_true by auto
 
+lemma fixpoint_is_equal_correct_externref_neq:
+  "\<not>is_equal (to_handle r1) (to_handle r2) \<longleftrightarrow> host_func_apply_impl s type0 fixpoint_is_equal 
+  [(V_ref (ConstRefExtern r1)), (V_ref (ConstRefExtern r2))] = Some(s, [V_num (ConstInt32 (I32.int_of_nat 0))])"
+  using fixpoint_is_equal_correct_handle_neq fixpoint_is_equal_impl by auto
 end
