wasm-proofs/Wasm-Proof/Init.thy
@@ -2,7 +2,8 @@ theory Init
   imports Host
 begin
 
-definition init :: "s" where "init = 
+definition init :: "s" where
+ "init = 
 \<lparr> funcs = 
 [(Func_host ([(T_ref T_ext_ref), (T_ref T_ext_ref)] _> [(T_num T_i32)]) (Host_func fixpoint_is_equal)),
 (Func_native 
@@ -22,7 +23,7 @@ datas = []
 (Call 0),
 (If (Tbv (Some (T_ref T_ext_ref)))
 [(Local_get 0)]
-[(Local_get 1)])])],
+[(Local_get 1)]) ]) ],
 tabs = [],
 mems = [],
 globs = [],
