wasm-proofs/Wasm-Proof/Wasm_Proof_Playground.thy
@@ -1,29 +1,100 @@
 theory Wasm_Proof_Playground 
-  imports WebAssembly_Dev.Wasm_Interpreter WebAssembly_Dev.Wasm WebAssembly_Dev.Wasm_Ast WebAssembly_Dev.Wasm_Interpreter_Properties
+  imports WebAssembly_Dev.Wasm_Interpreter WebAssembly_Dev.Wasm WebAssembly_Dev.Wasm_Ast
+  WebAssembly_Dev.Wasm_Countable
+  WebAssembly_Dev.Wasm_Base_Defs
+  Init
 begin
 
-lemma sc:
-"(app_binop_i Add (I32.int_of_nat 1) (I32.int_of_nat 2)) = Some (int_add (I32.int_of_nat 1) (I32.int_of_nat 2))" 
-  by (simp add: app_binop_i_def)
+(* Helper lemmas for int_eqz *)
+lemma se:
+  "\<not> int_eq (I32.int_of_nat (Suc 0)) 0"
+  by (simp add: I32.int_of_nat_def int_eq_i32_def Wasm_Ast.i32.Rep_i32_inject zero_i32_def I32.int_eq_def Wasm_Ast.i32.Abs_i32_inject)
 
-thm "I32.rep_abs"
-find_theorems name: "rep_abs" 
+lemma sf:
+  "int_eq (I32.int_of_nat 0) 0"
+  by (simp add: I32.int_eq_def I32.int_of_nat_def int_eq_i32.abs_eq zero_i32_def)
 
-lemma sd:
-"app_binop_i Add (I32.int_of_nat 1) (I32.int_of_nat 2) = Some (I32.int_of_nat 3)" 
+(* Given a fuel and depth that is enough to get to the result state, after run_iter, the result is a specific input argument *)
+lemma init_run_iter:
+  assumes "is_equal (to_handle r1) (to_handle r2)"
+  shows "run_iter (Suc (Suc (Suc (Suc (Suc (Suc (Suc (Suc (Suc (Suc (Suc (Suc n)))))))))))) (Config (Suc n') init (Frame_context (Redex [(V_ref (ConstRefExtern r2)), (V_ref (ConstRefExtern r1))] [Invoke 1] []) [] 0 empty_frame) []) = 
+     (let v_s = [V_ref (ConstRefExtern r1)]
+     in (Config (Suc n')
+         init
+         (Frame_context (Redex v_s [] []) [] 0 empty_frame) [],
+         RValue v_s))"
+  using fixpoint_is_equal_correct_externref[of r1 r2 init] assms
+  by (auto split: cl.splits simp add: n_zeros_def app_f_v_s_local_get_def app_f_call_def sfunc_ind_def typeof_def typeof_num_def init_def app_v_s_if_def se tb_tf_def)
+
+lemma init_run_iter_neq:
+  assumes "\<not>is_equal (to_handle r1) (to_handle r2)"
+  shows "run_iter (Suc (Suc (Suc (Suc (Suc (Suc (Suc (Suc (Suc (Suc (Suc (Suc n)))))))))))) (Config (Suc n') init (Frame_context (Redex [(V_ref (ConstRefExtern r2)), (V_ref (ConstRefExtern r1))] [Invoke 1] []) [] 0 empty_frame) []) = 
+     (let v_s = [V_ref (ConstRefExtern r2)]
+     in (Config (Suc n')
+         init
+         (Frame_context (Redex v_s [] []) [] 0 empty_frame) [],
+         RValue v_s))"
+  using fixpoint_is_equal_correct_externref_neq[of r1 r2 init] assms
+  by (auto split: cl.splits simp add: n_zeros_def app_f_v_s_local_get_def app_f_call_def sfunc_ind_def typeof_def typeof_num_def init_def app_v_s_if_def sf tb_tf_def)
+
+(* From the run_iter lemmas, one step out to the run_invoke lemmas *)
+lemma init_run_invoke:
+  assumes "is_equal (to_handle r1) (to_handle r2)" 
+  shows "run_invoke_v (Suc (Suc (Suc (Suc (Suc (Suc (Suc (Suc (Suc (Suc (Suc (Suc 0))))))))))))
+   (Suc 0) (init, [(V_ref (ConstRefExtern r1)), (V_ref (ConstRefExtern r2))], 1) = (init, RValue [V_ref (ConstRefExtern r1)])"
 proof -
-  have "int_add (I32.int_of_nat 1) (I32.int_of_nat 2) = I32.int_of_nat 3"
-    by (simp add: I32.int_add_def I32.int_of_nat_def int_add_i32_def I32.rep_abs)
-  then show ?thesis using sc by auto
+  have X: "run_iter (Suc (Suc (Suc (Suc (Suc (Suc (Suc (Suc (Suc (Suc (Suc (Suc 0)))))))))))) (Config (Suc 0) init (Frame_context (Redex [(V_ref (ConstRefExtern r2)), (V_ref (ConstRefExtern r1))] [Invoke 1] []) [] 0 empty_frame) []) = 
+     (let v_s = [V_ref (ConstRefExtern r1)]
+     in (Config (Suc 0)
+         init
+         (Frame_context (Redex v_s [] []) [] 0 empty_frame) [],
+         RValue v_s))"
+    using init_run_iter assms by auto
+
+  have Y: "rev [(V_ref (ConstRefExtern r1)), (V_ref (ConstRefExtern r2))] = [(V_ref (ConstRefExtern r2)), (V_ref (ConstRefExtern r1))]"
+    by auto
+
+  show ?thesis
+    apply (auto split: config.splits simp only: X run_invoke_v.simps Y case_prod_conv)
+    apply (auto split: config.splits)
+    apply (metis case_prod_conv config.case)
+    done
 qed
 
-lemma run_iter_with_locals:
-  "run_iter (Suc (Suc (Suc n)))
-             (Config d s 
-             (Frame_context (Redex [] [] [(Local_get 0), (Local_get 1), (Binop T_i32 (Binop_i Add))]) lcs nf 
-             (\<lparr>f_locs = [V_num (ConstInt32 (I32.int_of_nat 1)), V_num (ConstInt32 (I32.int_of_nat 2))], f_inst = inst \<rparr>)) fcs) =
-   run_iter n (Config d s 
-               (Frame_context (Redex [(V_num (ConstInt32 (I32.int_of_nat 3)))] [] []) lcs nf 
-               (\<lparr>f_locs = [V_num (ConstInt32 (I32.int_of_nat 1)), V_num (ConstInt32 (I32.int_of_nat 2))], f_inst = inst \<rparr>)) fcs)"
-  using app_f_v_s_local_get_def app_v_s_binop_def app_binop_def app_binop_i_v_def sd by auto
+lemma init_run_invoke_neq:
+  assumes "\<not>is_equal (to_handle r1) (to_handle r2)" 
+  shows "run_invoke_v (Suc (Suc (Suc (Suc (Suc (Suc (Suc (Suc (Suc (Suc (Suc (Suc 0))))))))))))
+   (Suc 0) (init, [(V_ref (ConstRefExtern r1)), (V_ref (ConstRefExtern r2))], 1) = (init, RValue [V_ref (ConstRefExtern r2)])"
+proof -
+  have X: "run_iter (Suc (Suc (Suc (Suc (Suc (Suc (Suc (Suc (Suc (Suc (Suc (Suc 0)))))))))))) (Config (Suc 0) init (Frame_context (Redex [(V_ref (ConstRefExtern r2)), (V_ref (ConstRefExtern r1))] [Invoke 1] []) [] 0 empty_frame) []) = 
+     (let v_s = [V_ref (ConstRefExtern r2)]
+     in (Config (Suc 0)
+         init
+         (Frame_context (Redex v_s [] []) [] 0 empty_frame) [],
+         RValue v_s))"
+    using init_run_iter_neq assms by auto
+
+  have Y: "rev [(V_ref (ConstRefExtern r1)), (V_ref (ConstRefExtern r2))] = [(V_ref (ConstRefExtern r2)), (V_ref (ConstRefExtern r1))]"
+    by auto
+
+  show ?thesis
+    apply (auto split: config.splits simp only: X run_invoke_v.simps Y case_prod_conv)
+    apply (auto split: config.splits)
+    apply (metis case_prod_conv config.case)
+    done
+qed
+
+fun isabelle_func :: "handle \<Rightarrow> handle \<Rightarrow> handle" where
+  "isabelle_func h1 h2 = (if (is_equal h1 h2) then h1 else h2)"
+
+(* Now we show that the function at index 1 is equivalent to the isabelle function such that there exists a fuel and depth such that for any pair of input handles, translating those to externrefs and invoking the function with the fuel and depth returns a result that is the same as translating the isabelle function output to an externref.*)
+lemma func_equiv:
+  "\<exists>f d s.
+   run_invoke_v f d 
+   (init, 
+   [V_ref (ConstRefExtern (to_externref h1)), 
+    V_ref (ConstRefExtern (to_externref h2))], 1) 
+   = (s, RValue [V_ref (ConstRefExtern (to_externref (isabelle_func h1 h2)))])"
+  by (metis init_run_invoke init_run_invoke_neq isabelle_func.simps to_handle_to_externref)
+
 end
